DequeSimplyTyped finished

theory/Deque/DequeSimplyTyped.v
@@ -21,8 +21,10 @@ Inductive color := Red | Yellow | Green.
    It can also be thought of as a set of colors. *)
 
 Definition color_constraint := color -> Prop.
-
 Implicit Type cc : color_constraint.
+
+Definition valid_c (P : color_constraint -> Prop) (c : color) : Prop :=
+  forall cc, cc c -> P cc.
 
 Definition red c := c = Red.
 Definition yellow c := c = Yellow.
@@ -41,6 +43,9 @@ Hint Unfold green_or_yellow : easy.
 Lemma red_is_not_green : ~ (Red = Green).
 Proof. intro; congruence. Qed.
 
+Lemma yellow_is_not_red : ~ (Yellow = Red).
+Proof. intro; congruence. Qed.
+
 Lemma red_or_yellow_is_not_green : ~ (Red = Green \/ Yellow = Green).
 Proof. intros [|]; congruence. Qed.
 
@@ -54,6 +59,7 @@ Proof. intros [|]; congruence. Qed.
 
 #[local] Hint Resolve
   red_is_not_green
+  yellow_is_not_red
   red_or_yellow_is_not_green
   yellow_is_not_green_or_red
   red_is_not_green_or_yellow
@@ -80,12 +86,18 @@ Arguments B4 {A}.
 Arguments B5 {A}.
 
 (* The buffered are colored according to their number of elements. *)
-Definition colored_buffer {A} cc (b : buffer A) : Prop :=
+Definition colored_buffer {A} (b : buffer A) (c : color) : Prop :=
   match b with
-  | B0 | B5 _ _ _ _ _ => cc Red
-  | B1 _ | B4 _ _ _ _ => cc Red \/ cc Yellow
+  | B0 | B5 _ _ _ _ _ => c = Red
+  | B1 _ | B4 _ _ _ _ => c = Red \/ c = Yellow
   | B2 _ _ | B3 _ _ _ => True
   end.
+
+(* All buffers can be colored red. *)
+Lemma colored_buffer_red {A} (b : buffer A) : colored_buffer b Red.
+Proof. destruct b; simpl; auto. Qed.
+
+#[local] Hint Resolve colored_buffer_red : easy.
 
 (* A type for packets. *)
 Inductive packet (A : Type) : Type -> Type :=
@@ -95,10 +107,10 @@ Arguments Hole {A}.
 Arguments Packet {A B}.
 
 (* A packet has the same color as its two buffers. *)
-Definition colored_packet {A B} cc (p : packet A B) : Prop :=
+Definition colored_packet {A B} (p : packet A B) (c : color) : Prop :=
   match p with
   | Hole => True
-  | Packet bp _ bs => colored_buffer cc bp /\ colored_buffer cc bs
+  | Packet bp _ bs => colored_buffer bp c /\ colored_buffer bs c
   end.
 
 (* Well-formedness of packets.
@@ -107,8 +119,9 @@ Definition colored_packet {A B} cc (p : packet A B) : Prop :=
 Fixpoint wf_packet {A B} (deep : Prop) (p : packet A B) : Prop :=
   match p with
   | Hole => deep
-  | Packet _ p' _ =>
-    ((deep /\ colored_packet yellow p) \/ ~deep) /\ wf_packet True p'
+  | Packet p pkt s =>
+    ((deep /\ colored_packet (Packet p pkt s) Yellow) \/ ~deep) /\
+    wf_packet True pkt
   end.
 
 (* A type for chains. *)
@@ -119,10 +132,10 @@ Arguments Ending {A}.
 Arguments Chain {A B}.
 
 (* A chain has the same color as its first packet. *)
-Definition colored_chain {A} cc (c : chain A) : Prop :=
+Definition colored_chain {A} (c : chain A) cc : Prop :=
   match c with
   | Ending _ => True
-  | Chain p _ => colored_packet cc p
+  | Chain p _ => exists c, cc c /\ colored_packet p c
   end.
 
 (* [regularity p] has type [color_constraint]. It is the color constraint
@@ -132,9 +145,9 @@ Definition regularity {A B} (p : packet A B) (c : color) : Prop :=
   | Hole => True
   | Packet _ _ _ =>
     (* A green packet must be followed with a green or red chain. *)
-    (colored_packet green p /\ green_or_red c) \/
+    (colored_packet p Green /\ green_or_red c) \/
     (* A yellow or red packet must be followed with a green chain. *)
-    green c
+    (~ colored_packet p Green /\ green c)
   end.
 
 Fixpoint wf_chain {A} (c : chain A) : Prop :=
@@ -144,7 +157,7 @@ Fixpoint wf_chain {A} (c : chain A) : Prop :=
     (* The top packet must be well-formed. *)
     wf_packet False p /\
     (* The packet [p] imposes a color constraint on the subchain [c]. *)
-    colored_chain (regularity p) c /\
+    colored_chain c (regularity p) /\
     (* The subchain must be well-formed. *)
     wf_chain c
   end.
@@ -155,9 +168,9 @@ Fixpoint wf_chain {A} (c : chain A) : Prop :=
    buffers with 4 or 5 elements are decomposed into [Overflow]. *)
 Inductive decompose (A : Type) : Type :=
   | Underflow : option A -> decompose A
-  | Ok : forall b : buffer A, colored_buffer green b -> decompose A
+  | Ok : forall b : buffer A, colored_buffer b Green -> decompose A
   | Overflow :
-      forall b : buffer A, colored_buffer green b -> A * A -> decompose A.
+      forall b : buffer A, colored_buffer b Green -> A * A -> decompose A.
 Arguments Underflow {A}.
 Arguments Ok {A}.
 Arguments Overflow {A}.
@@ -178,7 +191,7 @@ Arguments T {A}.
 
 Definition wf_deque {A} (d : deque A) : Prop :=
   match d with
-  | T c => colored_chain green_or_yellow c /\ wf_chain c
+  | T c => colored_chain c green_or_yellow /\ wf_chain c
   end.
 
 (* +------------------------------------------------------------------------+ *)
@@ -269,8 +282,10 @@ deque_seq (T c) := chain_seq c.
 
 Ltac unpack :=
   match goal with
-  | h: _ /\ _      |- _ => destruct h
-  | h: exists x, _ |- _ => destruct h
+  |                |- ~ _ => intro
+  | h: _ /\ _      |- _   => destruct h
+  | h: _ \/ _      |- _   => destruct h
+  | h: exists x, _ |- _   => destruct h
   end.
 
 Ltac deduce :=
@@ -280,7 +295,9 @@ Ltac crunch :=
   lazymatch goal with
   | |- _ /\ _ =>
       split; crunch
+  | |- _ \/ _ => try solve [left; crunch]; right; crunch
   | _ =>
+      deduce;
       try tauto;
       try congruence;
       try lia;
@@ -288,7 +305,13 @@ Ltac crunch :=
   end.
 
 Ltac easy :=
-  solve [ deduce; crunch ].
+  solve [ crunch ].
+
+Ltac pose_destruct p d Heq Hpos :=
+  remember d as tmp eqn: Htmp;
+  pose (p) as Hp; rewrite <-Htmp in Hp; simpl in Hp;
+  destruct tmp; simpl in *;
+  rename Htmp into Heq; rename Hp into Hpos.
 
 (* +------------------------------------------------------------------------+ *)
 (* |                                  Core                                  | *)
@@ -299,7 +322,7 @@ Proof. intro Hf. exfalso. apply Hf. exact tp. Qed.
 
 (* Pushes on a green buffer. *)
 Equations green_push {A}
-  (x : A) (b : buffer A) (cc : colored_buffer green b) : buffer A :=
+  (x : A) (b : buffer A) (cc : colored_buffer b Green) : buffer A :=
 green_push x (B2 a b)   _  := B3 x a b;
 green_push x (B3 a b c) _  := B4 x a b c;
 green_push _ _          cc := falsity cc _.
@@ -307,8 +330,8 @@ Next Obligation. easy. Qed.
 Next Obligation. easy. Qed.
 
 Lemma green_push_yellow {A}
-  (x : A) (b : buffer A) (cc : colored_buffer green b) :
-    colored_buffer yellow (green_push x b cc).
+  (x : A) (b : buffer A) (cc : colored_buffer b Green) :
+    colored_buffer (green_push x b cc) Yellow.
 Proof.
   destruct b; try (apply (falsity cc); simpl; easy).
   - reflexivity.
@@ -316,7 +339,7 @@ Proof.
 Qed.
 
 Lemma green_push_seq {A}
-  (x : A) (b : buffer A) (cc : colored_buffer green b) :
+  (x : A) (b : buffer A) (cc : colored_buffer b Green) :
     buffer_seq (green_push x b cc) = [x] ++ buffer_seq b.
 Proof.
   destruct b; try (apply (falsity cc); simpl; easy); reflexivity.
@@ -324,7 +347,7 @@ Qed.
 
 (* Injects on a green buffer. *)
 Equations green_inject {A}
-  (b : buffer A) (x : A) (cc : colored_buffer green b) : buffer A :=
+  (b : buffer A) (x : A) (cc : colored_buffer b Green) : buffer A :=
 green_inject (B2 a b)   x _  := B3 a b x;
 green_inject (B3 a b c) x _  := B4 a b c x;
 green_inject _          _ cc := falsity cc _.
@@ -332,8 +355,8 @@ Next Obligation. easy. Qed.
 Next Obligation. easy. Qed.
 
 Lemma green_inject_yellow {A}
-  (b : buffer A) (x : A) (cc : colored_buffer green b) :
-    colored_buffer yellow (green_inject b x cc).
+  (b : buffer A) (x : A) (cc : colored_buffer b Green) :
+    colored_buffer (green_inject b x cc) Yellow.
 Proof.
   destruct b; try (apply (falsity cc); simpl; easy).
   - reflexivity.
@@ -341,7 +364,7 @@ Proof.
 Qed.
 
 Lemma green_inject_seq {A}
-  (b : buffer A) (x : A) (cc : colored_buffer green b) :
+  (b : buffer A) (x : A) (cc : colored_buffer b Green) :
     buffer_seq (green_inject b x cc) = buffer_seq b ++ [x].
 Proof.
   destruct b; try (apply (falsity cc); simpl; easy); reflexivity.
@@ -349,7 +372,7 @@ Qed.
 
 (* Pops off a green buffer. *)
 Equations green_pop {A}
-  (b : buffer A) (cc : colored_buffer green b) : A * buffer A :=
+  (b : buffer A) (cc : colored_buffer b Green) : A * buffer A :=
 green_pop (B2 a b)   _  := (a, B1 b);
 green_pop (B3 a b c) _  := (a, B2 b c);
 green_pop _          cc := falsity cc _.
@@ -357,24 +380,25 @@ Next Obligation. easy. Qed.
 Next Obligation. easy. Qed.
 
 Lemma green_pop_yellow {A}
-  (b : buffer A) (cc : colored_buffer green b) :
-    colored_buffer yellow (snd (green_pop b cc)).
+  (b : buffer A) (cc : colored_buffer b Green) :
+    let '(x, b') := green_pop b cc in
+    colored_buffer b' Yellow.
 Proof.
   destruct b; try (apply (falsity cc); simpl; easy).
   - simpl. right. reflexivity.
   - reflexivity.
 Qed.
 
-Lemma green_pop_seq {A} (b : buffer A) (cc : colored_buffer green b) :
-    let '(x, b') := green_pop b cc in
-    [x] ++ buffer_seq b' = buffer_seq b.
+Lemma green_pop_seq {A} (b : buffer A) (cc : colored_buffer b Green) :
+  let '(x, b') := green_pop b cc in
+  [x] ++ buffer_seq b' = buffer_seq b.
 Proof.
   destruct b; try (apply (falsity cc); simpl; easy); reflexivity.
 Qed.
 
 (* Ejects off a green buffer. *)
 Equations green_eject {A}
-  (b : buffer A) (cc : colored_buffer green b) : buffer A * A :=
+  (b : buffer A) (cc : colored_buffer b Green) : buffer A * A :=
 green_eject (B2 a b)   _  := (B1 a, b);
 green_eject (B3 a b c) _  := (B2 a b, c);
 green_eject _          cc := falsity cc _.
@@ -382,24 +406,25 @@ Next Obligation. easy. Qed.
 Next Obligation. easy. Qed.
 
 Lemma green_eject_yellow {A}
-  (b : buffer A) (cc : colored_buffer green b) :
-    colored_buffer yellow (fst (green_eject b cc)).
+  (b : buffer A) (cc : colored_buffer b Green) :
+    let '(b', x) := green_eject b cc in
+    colored_buffer b' Yellow.
 Proof.
   destruct b; try (apply (falsity cc); simpl; easy).
   - simpl. right. reflexivity.
   - reflexivity.
 Qed.
 
-Lemma green_eject_seq {A} (b : buffer A) (cc : colored_buffer green b) :
-    let '(b', x) := green_eject b cc in
-    buffer_seq b' ++ [x] = buffer_seq b.
+Lemma green_eject_seq {A} (b : buffer A) (cc : colored_buffer b Green) :
+  let '(b', x) := green_eject b cc in
+  buffer_seq b' ++ [x] = buffer_seq b.
 Proof.
   destruct b; try (apply (falsity cc); simpl; easy); reflexivity.
 Qed.
 
 (* Pushes on a yellow buffer. *)
 Equations yellow_push {A}
-  (x : A) (b : buffer A) (cc : colored_buffer yellow b) : buffer A :=
+  (x : A) (b : buffer A) (cc : colored_buffer b Yellow) : buffer A :=
 yellow_push x (B1 a)       _  := B2 x a;
 yellow_push x (B2 a b)     _  := B3 x a b;
 yellow_push x (B3 a b c)   _  := B4 x a b c;
@@ -407,7 +432,7 @@ yellow_push x (B4 a b c d) _  := B5 x a b c d;
 yellow_push x _            cc := falsity cc _.
 
 Lemma yellow_push_seq {A}
-  (x : A) (b : buffer A) (cc : colored_buffer yellow b) :
+  (x : A) (b : buffer A) (cc : colored_buffer b Yellow) :
     buffer_seq (yellow_push x b cc) = [x] ++ buffer_seq b.
 Proof.
   destruct b; try (apply (falsity cc); simpl; easy); reflexivity.
@@ -415,7 +440,7 @@ Qed.
 
 (* Injects on a yellow buffer. *)
 Equations yellow_inject {A}
-  (b : buffer A) (x : A) (cc : colored_buffer yellow b) : buffer A :=
+  (b : buffer A) (x : A) (cc : colored_buffer b Yellow) : buffer A :=
 yellow_inject (B1 a)       x _  := B2 a x;
 yellow_inject (B2 a b)     x _  := B3 a b x;
 yellow_inject (B3 a b c)   x _  := B4 a b c x;
@@ -423,7 +448,7 @@ yellow_inject (B4 a b c d) x _  := B5 a b c d x;
 yellow_inject _            x cc := falsity cc _.
 
 Lemma yellow_inject_seq {A}
-  (b : buffer A) (x : A) (cc : colored_buffer yellow b) :
+  (b : buffer A) (x : A) (cc : colored_buffer b Yellow) :
     buffer_seq (yellow_inject b x cc) = buffer_seq b ++ [x].
 Proof.
   destruct b; try (apply (falsity cc); simpl; easy); reflexivity.
@@ -431,32 +456,32 @@ Qed.
 
 (* Pops off a yellow buffer. *)
 Equations yellow_pop {A}
-  (b : buffer A) (cc : colored_buffer yellow b) : A * buffer A :=
+  (b : buffer A) (cc : colored_buffer b Yellow) : A * buffer A :=
 yellow_pop (B1 a)       _  := (a, B0);
 yellow_pop (B2 a b)     _  := (a, B1 b);
 yellow_pop (B3 a b c)   _  := (a, B2 b c);
 yellow_pop (B4 a b c d) _  := (a, B3 b c d);
 yellow_pop _            cc := falsity cc _.
 
-Lemma yellow_pop_seq {A} (b : buffer A) (cc : colored_buffer yellow b) :
-    let '(x, b') := yellow_pop b cc in
-    [x] ++ buffer_seq b' = buffer_seq b.
+Lemma yellow_pop_seq {A} (b : buffer A) (cc : colored_buffer b Yellow) :
+  let '(x, b') := yellow_pop b cc in
+  [x] ++ buffer_seq b' = buffer_seq b.
 Proof.
   destruct b; try (apply (falsity cc); simpl; easy); reflexivity.
 Qed.
 
 (* Ejects off a yellow buffer. *)
 Equations yellow_eject {A}
-  (b : buffer A) (cc : colored_buffer yellow b) : buffer A * A :=
+  (b : buffer A) (cc : colored_buffer b Yellow) : buffer A * A :=
 yellow_eject (B1 a)       _  := (B0, a);
 yellow_eject (B2 a b)     _  := (B1 a, b);
 yellow_eject (B3 a b c)   _  := (B2 a b, c);
 yellow_eject (B4 a b c d) _  := (B3 a b c, d);
 yellow_eject _            cc := falsity cc _.
 
-Lemma yellow_eject_seq {A} (b : buffer A) (cc : colored_buffer yellow b) :
-    let '(b', x) := yellow_eject b cc in
-    buffer_seq b' ++ [x] = buffer_seq b.
+Lemma yellow_eject_seq {A} (b : buffer A) (cc : colored_buffer b Yellow) :
+  let '(b', x) := yellow_eject b cc in
+  buffer_seq b' ++ [x] = buffer_seq b.
 Proof.
   destruct b; try (apply (falsity cc); simpl; easy); reflexivity.
 Qed.
@@ -471,7 +496,7 @@ buffer_push x (B4 a b c d)   := Ending (B5 x a b c d);
 buffer_push x (B5 a b c d e) :=
     Chain (Packet (B3 x a b) Hole (B3 c d e)) (Ending B0).
 
-Lemma wf_buffer_push {A} (x : A) (b : buffer A) : wf_chain (buffer_push x b).
+Lemma buffer_push_wf {A} (x : A) (b : buffer A) : wf_chain (buffer_push x b).
 Proof.
   destruct b; simpl; try reflexivity.
   split; split; try reflexivity.
@@ -479,10 +504,10 @@ Proof.
 Qed.
 
 Lemma buffer_push_green {A} (x : A) (b : buffer A) :
-  colored_chain green (buffer_push x b).
+  forall cc, cc Green -> colored_chain (buffer_push x b) cc.
 Proof.
   destruct b; simpl; try reflexivity.
-  split; reflexivity.
+  exists Green; easy.
 Qed.
 
 Lemma buffer_push_seq {A} (x : A) (b : buffer A) :
@@ -499,7 +524,7 @@ buffer_inject (B4 a b c d) x   := Ending (B5 a b c d x);
 buffer_inject (B5 a b c d e) x :=
     Chain (Packet (B3 a b c) Hole (B3 d e x)) (Ending B0).
 
-Lemma wf_buffer_inject {A} (b : buffer A) (x : A) :
+Lemma buffer_inject_wf {A} (b : buffer A) (x : A) :
   wf_chain (buffer_inject b x).
 Proof.
   destruct b; simpl; try reflexivity.
@@ -508,10 +533,10 @@ Proof.
 Qed.
 
 Lemma buffer_inject_green {A} (b : buffer A) (x : A) :
-  colored_chain green (buffer_inject b x).
+  forall cc, cc Green -> colored_chain (buffer_inject b x) cc.
 Proof.
   destruct b; simpl; try reflexivity.
-  split; reflexivity.
+  exists Green; easy.
 Qed.
 
 Lemma buffer_inject_seq {A} (b : buffer A) (x : A) :
@@ -586,7 +611,7 @@ prefix23  None    (b, c) := B2 b c;
 prefix23 (Some a) (b, c) := B3 a b c.
 
 Lemma prefix23_green {A} (o : option A) (p : A * A) :
-  colored_buffer green (prefix23 o p).
+  colored_buffer (prefix23 o p) Green.
 Proof. destruct o; destruct p; reflexivity. Qed.
 
 Lemma prefix23_seq {A} (o : option A) (p : A * A) :
@@ -599,7 +624,7 @@ suffix23 (a, b)  None    := B2 a b;
 suffix23 (a, b) (Some c) := B3 a b c.
 
 Lemma suffix23_green {A} (p : A * A) (o : option A) :
-  colored_buffer green (suffix23 p o).
+  colored_buffer (suffix23 p o) Green.
 Proof. destruct p; destruct o; reflexivity. Qed.
 
 Lemma suffix23_seq {A} (p : A * A) (o : option A) :
@@ -612,7 +637,7 @@ suffix12 x  None    := B1 x;
 suffix12 x (Some y) := B2 x y.
 
 Lemma suffix12_yellow {A} (x : A) (o : option A) :
-  colored_buffer yellow (suffix12 x o).
+  colored_buffer (suffix12 x o) Yellow.
 Proof.
   destruct o; simpl.
   - reflexivity.
@@ -688,10 +713,11 @@ Proof. destruct b; reflexivity. Qed.
    obligations generated by [Equations]. *)
 #[export] Hint Rewrite <-app_assoc : rlist.
 #[export] Hint Rewrite app_nil_r : rlist.
+#[export] Hint Rewrite app_nil_l : rlist.
 #[export] Hint Rewrite flattenp_app : rlist.
 
 Lemma green_buffer_to_yellow_buffer {A} (b : buffer A) :
-  colored_buffer green b -> colored_buffer yellow b.
+  colored_buffer b Green -> colored_buffer b Yellow.
 Proof.
   intro cc.
   destruct b; try (apply (falsity cc); simpl; easy); reflexivity.
@@ -701,29 +727,25 @@ Qed.
    contained in them, and returns a green buffer and a yellow buffer of pairs.
    The order of elements is preserved. *)
 Equations green_prefix_concat {A}
-  (b1 : buffer A) (b2 : buffer (A * A)) (cc : colored_buffer green b2) :
+  (b1 : buffer A) (b2 : buffer (A * A)) (cc : colored_buffer b2 Green) :
   buffer A * buffer (A * A) :=
 green_prefix_concat b1 b2 cc with prefix_decompose b1 => {
   | Underflow opt with green_pop b2 cc => {
-    | (ab, b) with prefix23 opt ab => {
-      | prefix := (prefix, b) } };
+    | (ab, b) := (prefix23 opt ab, b) };
   | Ok b _ := (b, b2);
-  | Overflow b _ ab with green_push ab b2 cc => {
-    | suffix := (b, suffix) } }.
+  | Overflow b _ ab := (b, green_push ab b2 cc) }.
 
 Lemma green_prefix_concat_green_yellow {A}
-  (b1 : buffer A) (b2 : buffer (A * A)) (cc : colored_buffer green b2) :
+  (b1 : buffer A) (b2 : buffer (A * A)) (cc : colored_buffer b2 Green) :
     let '(b1', b2') := green_prefix_concat b1 b2 cc in
-    colored_buffer green b1' /\ colored_buffer yellow b2'.
+    colored_buffer b1' Green /\ colored_buffer b2' Yellow.
 Proof.
-  unfold green_prefix_concat. remember (prefix_decompose b1) as d.
-  destruct d; simpl.
-  - remember (green_pop b2 cc) as gp; destruct gp; simpl.
+  unfold green_prefix_concat.
+  destruct (prefix_decompose b1); simpl.
+  - pose_destruct (green_pop_yellow b2 cc) (green_pop b2 cc) Heq Hcol.
     split.
     + apply prefix23_green.
-    + replace (b) with (snd (green_pop b2 cc))
-        by (rewrite <-Heqgp; reflexivity).
-      apply green_pop_yellow.
+    + assumption.
   - split.
     + assumption.
     + apply green_buffer_to_yellow_buffer; assumption.
@@ -733,17 +755,14 @@ Proof.
 Qed.
 
 Lemma green_prefix_concat_seq {A}
-  (b1 : buffer A) (b2 : buffer (A * A)) (cc : colored_buffer green b2) :
+  (b1 : buffer A) (b2 : buffer (A * A)) (cc : colored_buffer b2 Green) :
     let '(b1', b2') := green_prefix_concat b1 b2 cc in
     buffer_seq b1  ++ flattenp (buffer_seq b2) =
     buffer_seq b1' ++ flattenp (buffer_seq b2').
 Proof.
   unfold green_prefix_concat.
-  remember (prefix_decompose b1) as d.
-  pose (prefix_decompose_seq b1) as Hpds; rewrite <-Heqd in Hpds; simpl in Hpds.
-  destruct d; simpl in *.
-  - remember (green_pop b2 cc) as gp; destruct gp; simpl.
-    pose (green_pop_seq b2 cc) as Hgps; rewrite <-Heqgp in Hgps.
+  pose_destruct (prefix_decompose_seq b1) (prefix_decompose b1) Heq Hseq.
+  - pose_destruct (green_pop_seq b2 cc) (green_pop b2 cc) Heq' Hseq'.
     rewrite prefix23_seq.
     hauto db:rlist.
   - hauto db:rlist.
@@ -755,16 +774,827 @@ Qed.
 (* Takes a green buffer of pairs and a buffer of any color, rearranges elements
    contained in them, and returns a yellow buffer of pairs and a green buffer.
    The order of elements is preserved. *)
-Equations green_suffix_concat {A C}
-  (b1 : buffer (A * A) green)
-  (b2 : buffer A C) :
-  { '(b1', b2') : buffer (A * A) yellow * buffer A green |
+Equations green_suffix_concat {A}
+  (b1 : buffer (A * A)) (cc : colored_buffer b1 Green) (b2 : buffer A) :
+  buffer (A * A) * buffer A :=
+green_suffix_concat b1 cc b2 with suffix_decompose b2 => {
+  | Underflow opt with green_eject b1 cc => {
+    | (b, ab) := (b, suffix23 ab opt) };
+  | Ok b _ := (b1, b);
+  | Overflow b _ ab := (green_inject b1 ab cc, b) }.
+
+Lemma green_suffix_concat_yellow_green {A}
+  (b1 : buffer (A * A)) (cc : colored_buffer b1 Green) (b2 : buffer A) :
+    let '(b1', b2') := green_suffix_concat b1 cc b2 in
+    colored_buffer b1' Yellow /\ colored_buffer b2' Green.
+Proof.
+  unfold green_suffix_concat.
+  destruct (suffix_decompose b2); simpl.
+  - pose_destruct (green_eject_yellow b1 cc) (green_eject b1 cc) Heq Hcol.
+    split.
+    + assumption.
+    + apply suffix23_green.
+  - split.
+    + apply green_buffer_to_yellow_buffer; assumption.
+    + assumption.
+  - split.
+    + apply green_inject_yellow.
+    + assumption.
+Qed.
+
+Lemma green_suffix_concat_seq {A}
+  (b1 : buffer (A * A)) (cc : colored_buffer b1 Green) (b2 : buffer A) :
+    let '(b1', b2') := green_suffix_concat b1 cc b2 in
     flattenp (buffer_seq b1)  ++ buffer_seq b2 =
-    flattenp (buffer_seq b1') ++ buffer_seq b2' } :=
-green_suffix_concat b1 b2 with suffix_decompose b2 => {
-  | ? Underflow opt with green_eject b1 => {
-    | ? (b, ab) with suffix23 ab opt => {
-      | ? suffix := ? (b, suffix) } };
-  | ? Ok b := ? (to_yellow b1, b);
-  | ? Overflow b ab with green_inject b1 ab => {
-    | ? prefix := ? (prefix, b) } }.
+    flattenp (buffer_seq b1') ++ buffer_seq b2'.
+Proof.
+  unfold green_suffix_concat.
+  pose_destruct (suffix_decompose_seq b2) (suffix_decompose b2) Heq Hseq.
+  - pose_destruct (green_eject_seq b1 cc) (green_eject b1 cc) Heq' Hseq'.
+    rewrite suffix23_seq.
+    hauto db:rlist.
+  - hauto db:rlist.
+  - destruct p; simpl.
+    rewrite green_inject_seq.
+    hauto db:rlist.
+Qed.
+
+(* Takes a buffer of any color and a yellow buffer of pairs, rearranges
+   elements contained in them, and returns a green buffer and a buffer of pairs
+   of any color.
+   The order of elements is preserved. *)
+Equations yellow_prefix_concat {A}
+  (b1 : buffer A) (b2 : buffer (A * A)) (cc : colored_buffer b2 Yellow) :
+  buffer A * buffer (A * A) :=
+yellow_prefix_concat b1 b2 cc with prefix_decompose b1 => {
+  | Underflow opt with yellow_pop b2 cc => {
+    | (ab, b) := (prefix23 opt ab, b) };
+  | Ok b _ := (b, b2);
+  | Overflow b _ ab := (b, yellow_push ab b2 cc) }.
+
+Lemma yellow_prefix_concat_green_red {A}
+  (b1 : buffer A) (b2 : buffer (A * A)) (cc : colored_buffer b2 Yellow) :
+    let '(b1', b2') := yellow_prefix_concat b1 b2 cc in
+    colored_buffer b1' Green.
+Proof.
+  unfold yellow_prefix_concat.
+  destruct (prefix_decompose b1); simpl.
+  - destruct (yellow_pop b2 cc); simpl.
+    apply prefix23_green.
+  - assumption.
+  - assumption.
+Qed.
+
+Lemma yellow_prefix_concat_seq {A}
+  (b1 : buffer A) (b2 : buffer (A * A)) (cc : colored_buffer b2 Yellow) :
+    let '(b1', b2') := yellow_prefix_concat b1 b2 cc in
+    buffer_seq b1  ++ flattenp (buffer_seq b2) =
+    buffer_seq b1' ++ flattenp (buffer_seq b2').
+Proof.
+  unfold yellow_prefix_concat.
+  pose_destruct (prefix_decompose_seq b1) (prefix_decompose b1) Heq Hseq.
+  - pose_destruct (yellow_pop_seq b2 cc) (yellow_pop b2 cc) Heq' Hseq'.
+    rewrite prefix23_seq.
+    hauto db:rlist.
+  - hauto db:rlist.
+  - destruct p; simpl.
+    rewrite yellow_push_seq.
+    hauto db:rlist.
+Qed.
+
+(* Takes a yellow buffer of pairs and a buffer of any color, rearranges
+   elements contained in them, and returns a buffer of pairs of any color and a
+   green buffer.
+   The order of elements is preserved. *)
+Equations yellow_suffix_concat {A}
+  (b1 : buffer (A * A)) (cc : colored_buffer b1 Yellow) (b2 : buffer A) :
+  buffer (A * A) * buffer A :=
+yellow_suffix_concat b1 cc b2 with suffix_decompose b2 => {
+  | Underflow opt with yellow_eject b1 cc => {
+    | (b, ab) := (b, suffix23 ab opt) };
+  | Ok b _ := (b1, b);
+  | Overflow b _ ab := (yellow_inject b1 ab cc, b) }.
+
+Lemma yellow_suffix_concat_red_green {A}
+  (b1 : buffer (A * A)) (cc : colored_buffer b1 Yellow) (b2 : buffer A) :
+    let '(b1', b2') := yellow_suffix_concat b1 cc b2 in
+    colored_buffer b2' Green.
+Proof.
+  unfold yellow_suffix_concat.
+  destruct (suffix_decompose b2); simpl.
+  - destruct (yellow_eject b1 cc); simpl.
+    apply suffix23_green.
+  - assumption.
+  - assumption.
+Qed.
+
+Lemma yellow_suffix_concat_seq {A}
+  (b1 : buffer (A * A)) (cc : colored_buffer b1 Yellow) (b2 : buffer A) :
+    let '(b1', b2') := yellow_suffix_concat b1 cc b2 in
+    flattenp (buffer_seq b1)  ++ buffer_seq b2 =
+    flattenp (buffer_seq b1') ++ buffer_seq b2'.
+Proof.
+  unfold yellow_suffix_concat.
+  pose_destruct (suffix_decompose_seq b2) (suffix_decompose b2) Heq Hseq.
+  - pose_destruct (yellow_eject_seq b1 cc) (yellow_eject b1 cc) Heq' Hseq'.
+    rewrite suffix23_seq.
+    hauto db:rlist.
+  - hauto db:rlist.
+  - destruct p; simpl.
+    rewrite yellow_inject_seq.
+    hauto db:rlist.
+Qed.
+
+(* Creates a green chain from 3 options. *)
+Equations chain_of_opt3 {A}
+  (o1 : option A) (o2 : option (A * A)) (o3 : option A) : chain A :=
+chain_of_opt3 None None None := Ending B0;
+chain_of_opt3 (Some a) None None := Ending (B1 a);
+chain_of_opt3 None None (Some a) := Ending (B1 a);
+chain_of_opt3 (Some a) None (Some b) := Ending (B2 a b);
+chain_of_opt3 None (Some (a, b)) None := Ending (B2 a b);
+chain_of_opt3 (Some a) (Some (b, c)) None := Ending (B3 a b c);
+chain_of_opt3 None (Some (a, b)) (Some c) := Ending (B3 a b c);
+chain_of_opt3 (Some a) (Some (b, c)) (Some d) := Ending (B4 a b c d).
+
+Lemma chain_of_opt3_wf {A}
+  (o1 : option A) (o2 : option (A * A)) (o3 : option A) :
+  wf_chain (chain_of_opt3 o1 o2 o3).
+Proof.
+  destruct o1; destruct o2; try destruct p; destruct o3; simpl; exact I.
+Qed.
+
+Lemma chain_of_opt3_green {A}
+  (o1 : option A) (o2 : option (A * A)) (o3 : option A) :
+  colored_chain (chain_of_opt3 o1 o2 o3) green.
+Proof.
+  destruct o1; destruct o2; try destruct p; destruct o3; simpl; exact I.
+Qed.
+
+Lemma chain_of_opt3_seq {A}
+  (o1 : option A) (o2 : option (A * A)) (o3 : option A) :
+  chain_seq (chain_of_opt3 o1 o2 o3) =
+    option_seq o1 ++ flattenp (option_seq o2) ++ option_seq o3.
+Proof.
+  destruct o1; destruct o2; try destruct p; destruct o3; simpl; hauto db:rlist.
+Qed.
+
+(* Takes a prefix buffer, a child buffer, and a suffix buffer, and rearranges
+   all elements contained in these buffers to form a green chain.
+   The order of elements is preserved. *)
+Equations make_small {A}
+  (b1 : buffer A) (b2 : buffer (A * A)) (b3 : buffer A) :
+  chain A :=
+make_small b1 b2 b3 with prefix_decompose b1, suffix_decompose b3 => {
+  | Underflow p1, Underflow s1 with buffer_unsandwich b2 => {
+    | Alone opt := chain_of_opt3 p1 opt s1 ;
+    | Sandwich ab rest cd :=
+      Chain (Packet (prefix23 p1 ab) Hole (suffix23 cd s1)) (Ending rest) };
+  | Underflow p1, Ok s1 _ with buffer_pop b2 => {
+    | None with p1 => {
+      | None := Ending s1;
+      | Some x := buffer_push x s1 };
+    | Some (cd, rest) :=
+      Chain (Packet (prefix23 p1 cd) Hole s1) (Ending rest) };
+  | Underflow p1, Overflow s1 _ ab with suffix_rot b2 ab => {
+    | (cd, center) :=
+      Chain (Packet (prefix23 p1 cd) Hole s1) (Ending center) };
+  | Ok p1 _, Underflow s1 with buffer_eject b2 => {
+    | None with s1 => {
+      | None := Ending p1;
+      | Some x := buffer_inject p1 x };
+    | Some (rest, ab) :=
+      Chain (Packet p1 Hole (suffix23 ab s1)) (Ending rest) };
+  | Ok p1 _, Ok s1 _ := Chain (Packet p1 Hole s1) (Ending b2);
+  | Ok p1 _, Overflow s1 _ ab :=
+    Chain (Packet p1 Hole s1) (buffer_inject b2 ab);
+  | Overflow p1 _ cd, Underflow s1 with prefix_rot cd b2 => {
+    | (center, ab) :=
+      Chain (Packet p1 Hole (suffix23 ab s1)) (Ending center) };
+  | Overflow p1 _ cd, Ok s1 _ := Chain (Packet p1 Hole s1) (buffer_push cd b2);
+  | Overflow p1 _ cd, Overflow s1 _ ab with buffer_halve b2 => {
+    | (x, rest) :=
+      Chain (Packet p1 (Packet (suffix12 cd x) Hole (B1 ab)) s1) (Ending rest) }
+}.
+
+Lemma make_small_wf {A}
+  (b1 : buffer A) (b2 : buffer (A * A)) (b3 : buffer A) :
+  wf_chain (make_small b1 b2 b3).
+Proof.
+  unfold make_small. unfold make_small_clause_1.
+  remember (prefix_decompose b1) as pd. remember (suffix_decompose b3) as sd.
+  destruct pd; destruct sd; simpl.
+  - destruct (buffer_unsandwich b2); simpl.
+    + apply chain_of_opt3_wf.
+    + auto.
+  - destruct (buffer_pop b2); simpl.
+    + destruct p as [cd rest]; simpl; auto.
+    + destruct o; simpl.
+      -- apply buffer_push_wf.
+      -- exact I.
+  - destruct (suffix_rot b2 p) as [cd center]; simpl; auto.
+  - destruct (buffer_eject b2); simpl.
+    + destruct p as [rest ab]; simpl; auto.
+    + destruct o; simpl.
+      -- apply buffer_inject_wf.
+      -- exact I.
+  - auto.
+  - split; auto; split.
+    + destruct b2; try exists Green; simpl; repeat split; left; easy.
+    + apply buffer_inject_wf.
+  - destruct (prefix_rot p b2) as [center ab]; simpl; auto.
+  - split; auto; split.
+    + destruct b2; try exists Green; simpl; repeat split; left; easy.
+    + apply buffer_push_wf.
+  - destruct (buffer_halve b2) as [x rest]; simpl.
+    split; auto; split; auto; split; auto.
+    left; split; auto; split; auto.
+    apply suffix12_yellow.
+Qed.
+
+Lemma make_small_green {A}
+  (b1 : buffer A) (b2 : buffer (A * A)) (b3 : buffer A) :
+  colored_chain (make_small b1 b2 b3) green.
+Proof.
+  unfold make_small. unfold make_small_clause_1.
+  remember (prefix_decompose b1) as pd. remember (suffix_decompose b3) as sd.
+  destruct pd; destruct sd; simpl.
+  - destruct (buffer_unsandwich b2); simpl.
+    + apply chain_of_opt3_green.
+    + exists Green; split; try easy; split.
+      -- apply prefix23_green.
+      -- apply suffix23_green.
+  - destruct (buffer_pop b2); simpl.
+    + destruct p as [cd rest]; simpl.
+      exists Green; split; try easy; split.
+      -- apply prefix23_green.
+      -- assumption.
+    + destruct o; simpl.
+      -- apply buffer_push_green. easy.
+      -- exact I.
+  - destruct (suffix_rot b2 p) as [cd center]; simpl.
+    exists Green; split; try easy; split.
+    + apply prefix23_green.
+    + assumption.
+  - destruct (buffer_eject b2); simpl.
+    + destruct p as [rest ab]; simpl.
+      exists Green; split; try easy; split.
+      -- assumption.
+      -- apply suffix23_green.
+    + destruct o; simpl.
+      -- apply buffer_inject_green. easy.
+      -- exact I.
+  - exists Green; split; try easy; split; assumption.
+  - exists Green; split; try easy; split; assumption.
+  - destruct (prefix_rot p b2) as [center ab]; simpl.
+    exists Green; split; try easy; split.
+    + assumption.
+    + apply suffix23_green.
+  - exists Green; split; try easy; split; assumption.
+  - destruct (buffer_halve b2) as [x rest]; simpl.
+    exists Green; split; try easy; split; assumption.
+Qed.
+
+Lemma make_small_seq {A}
+  (b1 : buffer A) (b2 : buffer (A * A)) (b3 : buffer A) :
+  chain_seq (make_small b1 b2 b3) =
+  buffer_seq b1 ++ flattenp (buffer_seq b2) ++ buffer_seq b3.
+Proof.
+  unfold make_small. unfold make_small_clause_1.
+  remember (prefix_decompose b1) as pd. remember (suffix_decompose b3) as sd.
+  pose (prefix_decompose_seq b1) as Hpds; rewrite <-Heqpd in Hpds; simpl in Hpds.
+  pose (suffix_decompose_seq b3) as Hsds; rewrite <-Heqsd in Hsds; simpl in Hsds.
+  destruct pd; destruct sd; simpl in *.
+  - remember (buffer_unsandwich b2) as bus.
+    pose (buffer_unsandwich_seq b2) as Hbuss; rewrite <-Heqbus in Hbuss; simpl in Hbuss.
+    destruct bus; simpl in *.
+    + rewrite chain_of_opt3_seq; simpl. hauto db:rlist.
+    + rewrite prefix23_seq. rewrite suffix23_seq. hauto db:rlist.
+  - remember (buffer_pop b2) as bp.
+    pose (buffer_pop_seq b2) as Hbps; rewrite <-Heqbp in Hbps; simpl in Hbps.
+    destruct bp; simpl in *.
+    + destruct p as [cd rest]; simpl. rewrite prefix23_seq. hauto db:rlist.
+    + destruct o; simpl in *.
+      -- rewrite buffer_push_seq. hauto db:rlist.
+      -- hauto db:rlist.
+  - remember (suffix_rot b2 p) as sr.
+    pose (suffix_rot_seq b2 p) as Hsrs; rewrite <-Heqsr in Hsrs; simpl in Hsrs.
+    destruct sr as [cd center]; simpl in *.
+    rewrite prefix23_seq.
+    replace (pair_seq cd) with (flattenp [cd]) by hauto.
+    rewrite Hpds; do 2 rewrite <-app_assoc; f_equal; rewrite app_nil_l.
+    rewrite Hsds; do 2 rewrite app_assoc; f_equal.
+    rewrite <-flattenp_app; rewrite <-Hsrs; rewrite flattenp_app.
+    hauto.
+  - remember (buffer_eject b2) as be.
+    pose (buffer_eject_seq b2)  as Hbes; rewrite <-Heqbe in Hbes; simpl in Hbes.
+    destruct be; simpl in *.
+    + destruct p as [rest ab]; simpl. hauto db:rlist.
+    + destruct o; simpl in *.
+      -- rewrite buffer_inject_seq. hauto db:rlist.
+      -- hauto db:rlist.
+  - hauto db:rlist.
+  - rewrite buffer_inject_seq. hauto db:rlist.
+  - remember (prefix_rot p b2) as pr.
+    pose (prefix_rot_seq p b2) as Hprs; rewrite <-Heqpr in Hprs; simpl in Hprs.
+    destruct pr as [center ab]; simpl in *.
+    rewrite suffix23_seq.
+    replace (pair_seq ab) with (flattenp [ab]) by hauto.
+    rewrite Hpds; rewrite <-app_assoc; f_equal.
+    rewrite Hsds; rewrite app_nil_l; do 2 rewrite app_assoc; f_equal.
+    rewrite <-flattenp_app; rewrite <-Hprs; rewrite flattenp_app.
+    hauto.
+  - rewrite buffer_push_seq. hauto db:rlist.
+  - remember (buffer_halve b2) as bh.
+    pose (buffer_halve_seq b2) as Hbhs; rewrite <-Heqbh in Hbhs; simpl in Hbhs.
+    destruct bh as [x rest]; simpl.
+    rewrite suffix12_seq.
+    hauto db:rlist.
+Qed.
+
+Lemma are_green {A} (p1 s1 : buffer A) :
+  (colored_buffer p1 Green /\ colored_buffer s1 Green) +
+  ~ (colored_buffer p1 Green /\ colored_buffer s1 Green).
+Proof.
+  destruct p1; destruct s1; try (left; easy); right; easy.
+Qed.
+
+Lemma are_yellow {A} (p1 s1 : buffer A) :
+  (colored_buffer p1 Yellow /\ colored_buffer s1 Yellow) +
+  ~ (colored_buffer p1 Yellow /\ colored_buffer s1 Yellow).
+Proof.
+  destruct p1; destruct s1; try (left; easy); right; easy.
+Qed.
+
+(* Makes a red chain green. *)
+Equations ensure_green {A} (c : chain A) : chain A :=
+ensure_green (Chain (Packet p1 Hole s1) (Ending b)) := make_small p1 b s1;
+ensure_green (Chain (Packet p1 Hole s1) (Chain (Packet p2 p s2) c))
+  with are_green p1 s1 => {
+  | inl _ := Chain (Packet p1 Hole s1) (Chain (Packet p2 p s2) c);
+  | inr _ with are_green p2 s2 => {
+    | inl (conj p2g s2g)
+      with green_prefix_concat p1 p2 p2g, green_suffix_concat s2 s2g s1 => {
+      | (p1', p2'), (s2', s1') :=
+        Chain (Packet p1' (Packet p2' p s2') s1') c };
+    | inr _ := Chain (Packet p1 Hole s1) (Chain (Packet p2 p s2) c) } };
+ensure_green (Chain (Packet p1 (Packet p2 p s2) s1) c)
+  with are_green p1 s1 => {
+  | inl _ => Chain (Packet p1 (Packet p2 p s2) s1) c
+  | inr _ with are_yellow p2 s2 => {
+    | inl (conj p2y s2y)
+      with yellow_prefix_concat p1 p2 p2y, yellow_suffix_concat s2 s2y s1 => {
+      | (p1', p2'), (s2', s1') :=
+        Chain (Packet p1' Hole s1') (Chain (Packet p2' p s2') c) }
+    | inr _ := Chain (Packet p1 (Packet p2 p s2) s1) c } };
+ensure_green c := c.
+
+Lemma colored_buffer_split {A : Type} (b1 b2 : buffer A) cc1 cc2 :
+  forall c, cc1 c -> cc2 c ->
+    (colored_buffer b1 c /\ colored_buffer b2 c) /\ cc1 c \/
+    ~ (colored_buffer b1 c /\ colored_buffer b2 c) /\ cc2 c.
+Proof.
+  intros c cc1c cc2c.
+  destruct b1; destruct b2; destruct c; simpl; easy.
+Qed.
+
+Lemma ensure_green_wf {A} (c : chain A) (c_wf : wf_chain c) :
+  wf_chain (ensure_green c).
+Proof.
+  destruct c; simpl; auto.
+  destruct p as [|B p1 pkt s1]; simpl.
+  - apply (falsity c_wf). unfold wf_chain, wf_packet.
+    apply proj1.
+  - destruct pkt as [|B p2 pkt s2]; simpl.
+    + destruct c as [|B pkt c]; try apply make_small_wf.
+      destruct pkt as [|B p2 pkt s2]; try easy.
+      destruct (are_green p1 s1) as [[p1g s1g] | np1s1g]; try exact c_wf; simpl.
+      destruct (are_green p2 s2) as [[p2g s2g] | np2s2g]; try exact c_wf; simpl.
+      pose_destruct (green_prefix_concat_green_yellow p1 p2 p2g) (green_prefix_concat p1 p2 p2g) Heqp cbp.
+      pose_destruct (green_suffix_concat_yellow_green s2 s2g s1) (green_suffix_concat s2 s2g s1) Heqs cbs.
+      destruct cbp as [p1'g p2'y]; destruct cbs as [s2'y s1'g].
+      destruct c_wf as [p1_wf [cc2 [[p2c p2_wf] [ccc c_wf]]]].
+      repeat split; auto.
+      destruct c as [|C pkt' c]; auto.
+      destruct ccc as [col [[[Ht Hgr] | [Hf Hg]] colpkt]]; simpl in *.
+      -- exists col; easy.
+      -- easy.
+    + destruct (are_green p1 s1) as [[p1g s1g] | np1s1g]; try exact c_wf; simpl.
+      destruct (are_yellow p2 s2) as [[p2y s2y] | ny]; try exact c_wf; simpl.
+      pose_destruct (yellow_prefix_concat_green_red p1 p2 p2y) (yellow_prefix_concat p1 p2 p2y) Heqp p1g.
+      pose_destruct (yellow_suffix_concat_red_green s2 s2y s1) (yellow_suffix_concat s2 s2y s1) Heqs s1g.
+      destruct c_wf as [[p1_wf [p2_wf pkt_wf]] [ccc c_wf]]; simpl.
+      repeat split; auto.
+      -- exists Red; split; try left; easy.
+      -- repeat split; try easy.
+        destruct c as [|p3 pkt' s3]; auto; simpl in *.
+        exists Green; split.
+        ++ apply colored_buffer_split; easy.
+        ++ destruct ccc as [col [[[Hf Hgr] | [Hn Hg]] colpkt]]; easy.
+Qed.
+
+Lemma ensure_green_green {A} (c : chain A) (c_wf : wf_chain c) :
+  colored_chain (ensure_green c) green.
+Proof.
+  destruct c; simpl; auto.
+  destruct p as [|B p1 pkt s1]; simpl.
+  - apply (falsity c_wf). unfold wf_chain, wf_packet.
+    apply proj1.
+  - destruct pkt as [|B p2 pkt s2]; simpl.
+    + destruct c as [|B pkt c]; try apply make_small_green.
+      destruct pkt as [|B p2 pkt s2]; try easy.
+      destruct (are_green p1 s1) as [[p1g s1g] | np1s1g]; try easy; simpl.
+      destruct (are_green p2 s2) as [[p2g s2g] | np2s2g]; simpl.
+      -- pose_destruct (green_prefix_concat_green_yellow p1 p2 p2g) (green_prefix_concat p1 p2 p2g) Heqp cbp.
+         pose_destruct (green_suffix_concat_yellow_green s2 s2g s1) (green_suffix_concat s2 s2g s1) Heqs cbs.
+         exists Green; easy.
+      -- destruct c_wf as [p1_wf [[col [[[Hf Hgr] | [Ht Hg]] colpkt]] c_wf]].
+         ++ easy.
+         ++ unfold green in Hg; subst; easy.
+    + destruct (are_green p1 s1) as [[p1g s1g] | np1s1g]; try easy; simpl.
+      destruct (are_yellow p2 s2) as [[p2y s2y] | np2s2y]; try easy; simpl.
+      pose_destruct (yellow_prefix_concat_green_red p1 p2 p2y) (yellow_prefix_concat p1 p2 p2y) Heqp p1g.
+      pose_destruct (yellow_suffix_concat_red_green s2 s2y s1) (yellow_suffix_concat s2 s2y s1) Heqs s1g.
+      easy.
+Qed.
+
+Lemma ensure_green_seq {A} (c : chain A) (c_wf : wf_chain c) :
+  chain_seq (ensure_green c) = chain_seq c.
+Proof.
+  destruct c; simpl; auto.
+  destruct p as [|B p1 pkt s1]; simpl.
+  - apply (falsity c_wf). unfold wf_chain, wf_packet.
+    apply proj1.
+  - destruct pkt as [|B p2 pkt s2]; simpl.
+    + destruct c as [|B pkt c]; try apply make_small_seq.
+      destruct pkt as [|B p2 pkt s2]; try easy.
+      destruct (are_green p1 s1) as [[p1g s1g] | np1s1g]; try easy; simpl.
+      destruct (are_green p2 s2) as [[p2g s2g] | np2s2g]; try easy; simpl.
+      pose_destruct (green_prefix_concat_seq p1 p2 p2g) (green_prefix_concat p1 p2 p2g) Heqp Hseqp.
+      pose_destruct (green_suffix_concat_seq s2 s2g s1) (green_suffix_concat s2 s2g s1) Heqs Hseqs.
+      repeat rewrite flattenp_app.
+      repeat rewrite app_assoc.
+      rewrite Hseqp.
+      repeat rewrite <-app_assoc.
+      do 3 f_equal.
+      easy.
+    + destruct (are_green p1 s1) as [[p1g s1g] | np1s1g]; try easy; simpl.
+      destruct (are_yellow p2 s2) as [[p2y s2y] | np2s2y]; try easy; simpl.
+      pose_destruct (yellow_prefix_concat_seq p1 p2 p2y) (yellow_prefix_concat p1 p2 p2y) Heqp Hseqp.
+      pose_destruct (yellow_suffix_concat_seq s2 s2y s1) (yellow_suffix_concat s2 s2y s1) Heqs Hseqs.
+      repeat rewrite flattenp_app.
+      repeat rewrite app_assoc.
+      rewrite Hseqp.
+      repeat rewrite <-app_assoc.
+      do 3 f_equal.
+      easy.
+Qed.
+
+(* +------------------------------------------------------------------------+ *)
+(* |                               Operations                               | *)
+(* +------------------------------------------------------------------------+ *)
+
+(* The empty deque. *)
+Equations empty {A : Type} : deque A :=
+empty := T (Ending B0).
+
+Lemma empty_wf {A} : wf_deque (@empty A).
+Proof. easy. Qed.
+
+Lemma empty_seq {A} : deque_seq (@empty A) = [].
+Proof. reflexivity. Qed.
+
+(* Pushes on a deque. *)
+Equations push {A : Type} (x : A) (d : deque A) : deque A :=
+push x (T (Ending b)) := T (buffer_push x b);
+push x (T (Chain (Packet p pkt s) c)) with are_green p s => {
+  | inl (conj pg _) :=
+    T (Chain (Packet (green_push x p pg) pkt s) (ensure_green c));
+  | inr _ with are_yellow p s => {
+    | inl (conj py _) :=
+      T (ensure_green (Chain (Packet (yellow_push x p py) pkt s) c));
+    | inr _ := T (Chain (Packet p pkt s) c) } };
+push _ d := d.
+
+Lemma chain_green_to_green_or_yellow {A} (c : chain A) :
+  colored_chain c green -> colored_chain c green_or_yellow.
+Proof. intro ccg. destruct c; easy. Qed.
+
+Lemma regularity_green {A B} (pkt : packet A B) : (regularity pkt) Green.
+Proof.
+  destruct pkt; try easy; simpl.
+  destruct (are_green b b0) as [[bg b0g] | nbb0g]; easy.
+Qed.
+
+Lemma chain_green_to_regularity {A B} (c : chain B) (pkt : packet A B) :
+  colored_chain c green -> colored_chain c (regularity pkt).
+Proof.
+  intro ccg.
+  destruct c; auto; simpl in *.
+  destruct ccg as [col [colg colpkt]].
+  exists col; split; auto.
+  unfold green in colg; subst.
+  apply regularity_green.
+Qed.
+
+Lemma push_wf {A} (x : A) (d : deque A) (d_wf : wf_deque d) :
+  wf_deque (push x d).
+Proof.
+  destruct d. destruct c as [|_ [|B p pkt s] c]; simpl.
+  - split.
+    + apply buffer_push_green. easy.
+    + apply buffer_push_wf.
+  - destruct d_wf as [cc [pkt_wf rest]].
+    simpl in pkt_wf. destruct pkt_wf.
+  - destruct (are_green p s) as [[pg sg] | npsg]; simpl in *.
+    + destruct d_wf as [[col [colgy [pgy sgy]]] [[psy pkt_wf] [ccc c_wf]]].
+      repeat split; auto.
+      -- exists Yellow; repeat split; try easy.
+         ++ apply green_push_yellow.
+         ++ apply green_buffer_to_yellow_buffer. easy.
+      -- apply chain_green_to_regularity.
+         apply ensure_green_green.
+         exact c_wf.
+      -- apply ensure_green_wf.
+         exact c_wf.
+    + destruct (are_yellow p s) as [[py sy] | npsy]; try exact d_wf.
+      destruct d_wf as [[col [colgy [pgy sgy]]] [[psy pkt_wf] [ccc c_wf]]].
+      assert (wf_chain (Chain (Packet (yellow_push x p py) pkt s) c)) as pc_wf.
+      -- repeat split; auto.
+         destruct c; auto.
+         destruct ccc as [col' [[[psg grcol'] | [_ gcol']] pktcol']].
+         ++ exfalso. apply npsg. exact psg.
+         ++ exists Green; split; try easy.
+            apply regularity_green.
+      -- repeat split; auto.
+         ++ apply chain_green_to_green_or_yellow.
+            apply ensure_green_green.
+            exact pc_wf.
+         ++ apply ensure_green_wf.
+            exact pc_wf.
+Qed.
+
+Lemma push_seq {A} (x : A) (d : deque A) (d_wf : wf_deque d) :
+  deque_seq (push x d) = [x] ++ deque_seq d.
+Proof.
+  destruct d. destruct c as [|_ [|B p pkt s] c]; simpl.
+  - apply buffer_push_seq.
+  - destruct d_wf as [cc [pkt_wf rest]].
+    simpl in pkt_wf. destruct pkt_wf.
+  - destruct (are_green p s) as [[pg sg] | npsg]; simpl in *.
+    + rewrite green_push_seq.
+      rewrite ensure_green_seq; easy.
+    + destruct (are_yellow p s) as [[py sy] | npsy].
+      -- unfold push_clause_2_clause_2.
+         rewrite deque_seq_equation_1.
+         rewrite ensure_green_seq; simpl.
+         ++ rewrite yellow_push_seq. easy.
+         ++ destruct d_wf as [[col [colgy [pgy sgy]]] [[psy pkt_wf] [ccc c_wf]]].
+            repeat split; auto.
+            destruct c; auto.
+            destruct ccc as [col' [[[psg grcol'] | [_ gcol']] pktcol']].
+            --- exfalso. apply npsg. exact psg.
+            --- exists Green; split; try easy.
+                apply regularity_green.
+      -- destruct d_wf as [[col [colgy [pgy sgy]]] [[psy pkt_wf] [ccc c_wf]]].
+         destruct colgy; subst; easy.
+Qed.
+
+(* Injects on a deque. *)
+Equations inject {A : Type} (d : deque A) (x : A) : deque A :=
+inject (T (Ending b)) x := T (buffer_inject b x);
+inject (T (Chain (Packet p pkt s) c)) x with are_green p s => {
+  | inl (conj _ sg) :=
+    T (Chain (Packet p pkt (green_inject s x sg)) (ensure_green c));
+  | inr _ with are_yellow p s => {
+    | inl (conj _ sy) :=
+      T (ensure_green (Chain (Packet p pkt (yellow_inject s x sy)) c));
+    | inr _ := T (Chain (Packet p pkt s) c) } };
+inject d _ := d.
+
+Lemma inject_wf {A} (d : deque A) (x : A) (d_wf : wf_deque d) :
+  wf_deque (inject d x).
+Proof.
+  destruct d. destruct c as [|_ [|B p pkt s] c]; simpl.
+  - split.
+    + apply buffer_inject_green. easy.
+    + apply buffer_inject_wf.
+  - destruct d_wf as [cc [pkt_wf rest]].
+    simpl in pkt_wf. destruct pkt_wf.
+  - destruct (are_green p s) as [[pg sg] | npsg]; simpl in *.
+    + destruct d_wf as [[col [colgy [pgy sgy]]] [[psy pkt_wf] [ccc c_wf]]].
+      repeat split; auto.
+      -- exists Yellow; repeat split; try easy.
+         ++ apply green_buffer_to_yellow_buffer. easy.
+         ++ apply green_inject_yellow.
+      -- apply chain_green_to_regularity.
+         apply ensure_green_green.
+         exact c_wf.
+      -- apply ensure_green_wf.
+         exact c_wf.
+    + destruct (are_yellow p s) as [[py sy] | npsy]; try exact d_wf.
+      destruct d_wf as [[col [colgy [pgy sgy]]] [[psy pkt_wf] [ccc c_wf]]].
+      assert (wf_chain (Chain (Packet p pkt (yellow_inject s x sy)) c)) as pc_wf.
+      -- repeat split; auto.
+         destruct c; auto.
+         destruct ccc as [col' [[[psg grcol'] | [_ gcol']] pktcol']].
+         ++ exfalso. apply npsg. exact psg.
+         ++ exists Green; split; try easy.
+            apply regularity_green.
+      -- repeat split; auto.
+         ++ apply chain_green_to_green_or_yellow.
+            apply ensure_green_green.
+            exact pc_wf.
+         ++ apply ensure_green_wf.
+            exact pc_wf.
+Qed.
+
+Lemma inject_seq {A} (d : deque A) (x : A) (d_wf : wf_deque d) :
+  deque_seq (inject d x) = deque_seq d ++ [x].
+Proof.
+  destruct d. destruct c as [|_ [|B p pkt s] c]; simpl.
+  - apply buffer_inject_seq.
+  - destruct d_wf as [cc [pkt_wf rest]].
+    simpl in pkt_wf. destruct pkt_wf.
+  - destruct (are_green p s) as [[pg sg] | npsg]; simpl in *.
+    + rewrite green_inject_seq.
+      rewrite ensure_green_seq; hauto db:rlist.
+    + destruct (are_yellow p s) as [[py sy] | npsy].
+      -- unfold inject_clause_2_clause_2.
+         rewrite deque_seq_equation_1.
+         rewrite ensure_green_seq; simpl.
+         ++ rewrite yellow_inject_seq; hauto db:rlist.
+         ++ destruct d_wf as [[col [colgy [pgy sgy]]] [[psy pkt_wf] [ccc c_wf]]].
+            repeat split; auto.
+            destruct c; auto.
+            destruct ccc as [col' [[[psg grcol'] | [_ gcol']] pktcol']].
+            --- exfalso. apply npsg. exact psg.
+            --- exists Green; split; try easy.
+                apply regularity_green.
+      -- destruct d_wf as [[col [colgy [pgy sgy]]] [[psy pkt_wf] [ccc c_wf]]].
+         destruct colgy; subst; easy.
+Qed.
+
+(* Pops off a deque. *)
+Equations pop {A : Type} (d : deque A) : option (A * deque A) :=
+pop (T (Ending b)) with buffer_pop b => {
+  | None := None;
+  | Some (x, b') := Some (x, T (Ending b')) };
+pop (T (Chain (Packet p pkt s) c)) with are_green p s => {
+  | inl (conj pg _) with green_pop p pg => { | (x, p') :=
+    Some (x, T (Chain (Packet p' pkt s) (ensure_green c))) };
+  | inr _ with are_yellow p s => {
+    | inl (conj py _) with yellow_pop p py => { | (x, p') :=
+      Some (x, T (ensure_green (Chain (Packet p' pkt s) c))) };
+    | inr _ := None } };
+pop d := None.
+
+Lemma pop_wf {A} (d : deque A) (d_wf : wf_deque d) :
+  match pop d with
+  | None => True
+  | Some (_, d') => wf_deque d'
+  end.
+Proof.
+  destruct d. destruct c as [|_ [|B p pkt s] c]; simpl.
+  - destruct (buffer_pop b) as [[x b']|]; easy.
+  - easy.
+  - destruct (are_green p s) as [[pg sg] | npsg]; simpl in *.
+    + destruct d_wf as [[col [colgy [pgy sgy]]] [[psy pkt_wf] [ccc c_wf]]].
+      pose_destruct (green_pop_yellow p pg) (green_pop p pg) Heq Hcol; simpl.
+      repeat split; auto.
+      -- exists Yellow; repeat split; try easy.
+         apply green_buffer_to_yellow_buffer. easy.
+      -- apply chain_green_to_regularity.
+         apply ensure_green_green.
+         exact c_wf.
+      -- apply ensure_green_wf.
+         exact c_wf.
+    + destruct (are_yellow p s) as [[py sy] | npsy]; simpl; auto.
+      destruct d_wf as [[col [colgy [pgy sgy]]] [[psy pkt_wf] [ccc c_wf]]].
+      destruct (yellow_pop p py) as [x p'] eqn: Hyp.
+      assert (wf_chain (Chain (Packet p' pkt s) c)) as pc_wf.
+      -- repeat split; auto.
+         destruct c; auto.
+         apply chain_green_to_regularity.
+         destruct ccc as [col' [[[psg grcol'] | [_ gcol']] pktcol']]; easy.
+      -- split.
+         ++ apply chain_green_to_green_or_yellow.
+            apply ensure_green_green.
+            apply pc_wf.
+         ++ apply ensure_green_wf.
+            apply pc_wf.
+Qed.
+
+Lemma pop_seq {A} (d : deque A) (d_wf : wf_deque d) :
+  deque_seq d = match pop d with
+                | None => []
+                | Some (x, d') => [x] ++ deque_seq d'
+                end.
+Proof.
+  destruct d. destruct c as [|_ [|B p pkt s] c]; simpl.
+  - pose_destruct (buffer_pop_seq b) (buffer_pop b) Heq Hseq; auto.
+    destruct p. easy.
+  - easy.
+  - destruct (are_green p s) as [[pg sg] | npsg]; simpl in *.
+    + destruct d_wf as [[col [colgy [pgy sgy]]] [[psy pkt_wf] [ccc c_wf]]].
+      pose_destruct (green_pop_seq p pg) (green_pop p pg) Heq Hseq; simpl.
+      rewrite ensure_green_seq; auto.
+      hauto db:rlist.
+    + destruct (are_yellow p s) as [[py sy] | npsy]; simpl.
+      -- unfold pop_clause_2_clause_2_clause_1.
+         remember (yellow_pop p py) as tmp.
+         pose (yellow_pop_seq p py) as Hseq; rewrite <-Heqtmp in Hseq.
+         destruct tmp as [x p'].
+         rewrite deque_seq_equation_1.
+         rewrite ensure_green_seq.
+         ++ hauto db:rlist.
+         ++ destruct d_wf as [[col [colgy [pgy sgy]]] [[psy pkt_wf] [ccc c_wf]]].
+            repeat split; auto.
+            destruct c; auto.
+            apply chain_green_to_regularity.
+            destruct ccc as [col' [[[psg grcol'] | [_ gcol']] pktcol']]; easy.
+      -- destruct d_wf as [[col [colgy [pgy sgy]]] [[psy pkt_wf] [ccc c_wf]]].
+         destruct col; unfold green_or_yellow in colgy; easy.
+Qed.
+
+(* Ejects off a deque. *)
+Equations eject {A : Type} (d : deque A) : option (deque A * A) :=
+eject (T (Ending b)) with buffer_eject b => {
+  | None := None;
+  | Some (b', x) := Some (T (Ending b'), x) };
+eject (T (Chain (Packet p pkt s) c)) with are_green p s => {
+  | inl (conj _ sg) with green_eject s sg => { | (s', x) :=
+    Some (T (Chain (Packet p pkt s') (ensure_green c)), x) };
+  | inr _ with are_yellow p s => {
+    | inl (conj _ sy) with yellow_eject s sy => { | (s', x) :=
+      Some (T (ensure_green (Chain (Packet p pkt s') c)), x) };
+    | inr _ := None } };
+eject d := None.
+
+Lemma eject_wf {A} (d : deque A) (d_wf : wf_deque d) :
+  match eject d with
+  | None => True
+  | Some (d', _) => wf_deque d'
+  end.
+Proof.
+  destruct d. destruct c as [|_ [|B p pkt s] c]; simpl.
+  - destruct (buffer_eject b) as [[x b']|]; easy.
+  - easy.
+  - destruct (are_green p s) as [[pg sg] | npsg]; simpl in *.
+    + destruct d_wf as [[col [colgy [pgy sgy]]] [[psy pkt_wf] [ccc c_wf]]].
+      pose_destruct (green_eject_yellow s sg) (green_eject s sg) Heq Hcol; simpl.
+      repeat split; auto.
+      -- exists Yellow; repeat split; try easy.
+         apply green_buffer_to_yellow_buffer. easy.
+      -- apply chain_green_to_regularity.
+         apply ensure_green_green.
+         exact c_wf.
+      -- apply ensure_green_wf.
+         exact c_wf.
+    + destruct (are_yellow p s) as [[py sy] | npsy]; simpl; auto.
+      destruct d_wf as [[col [colgy [pgy sgy]]] [[psy pkt_wf] [ccc c_wf]]].
+      destruct (yellow_eject s sy) as [s' x] eqn: Hyp.
+      assert (wf_chain (Chain (Packet p pkt s') c)) as pc_wf.
+      -- repeat split; auto.
+         destruct c; auto.
+         apply chain_green_to_regularity.
+         destruct ccc as [col' [[[psg grcol'] | [_ gcol']] pktcol']]; easy.
+      -- split.
+         ++ apply chain_green_to_green_or_yellow.
+            apply ensure_green_green.
+            apply pc_wf.
+         ++ apply ensure_green_wf.
+            apply pc_wf.
+Qed.
+
+Lemma eject_seq {A} (d : deque A) (d_wf : wf_deque d) :
+  deque_seq d = match eject d with
+                | None => []
+                | Some (d', x) => deque_seq d' ++ [x]
+                end.
+Proof.
+  destruct d. destruct c as [|_ [|B p pkt s] c]; simpl.
+  - pose_destruct (buffer_eject_seq b) (buffer_eject b) Heq Hseq; auto.
+    destruct p. easy.
+  - easy.
+  - destruct (are_green p s) as [[pg sg] | npsg]; simpl in *.
+    + destruct d_wf as [[col [colgy [pgy sgy]]] [[psy pkt_wf] [ccc c_wf]]].
+      pose_destruct (green_eject_seq s sg) (green_eject s sg) Heq Hseq; simpl.
+      rewrite ensure_green_seq; auto.
+      hauto db:rlist.
+    + destruct (are_yellow p s) as [[py sy] | npsy]; simpl.
+      -- unfold eject_clause_2_clause_2_clause_1.
+         remember (yellow_eject s sy) as tmp.
+         pose (yellow_eject_seq s sy) as Hseq; rewrite <-Heqtmp in Hseq.
+         destruct tmp as [x s'].
+         rewrite deque_seq_equation_1.
+         rewrite ensure_green_seq.
+         ++ hauto db:rlist.
+         ++ destruct d_wf as [[col [colgy [pgy sgy]]] [[psy pkt_wf] [ccc c_wf]]].
+            repeat split; auto.
+            destruct c; auto.
+            apply chain_green_to_regularity.
+            destruct ccc as [col' [[[psg grcol'] | [_ gcol']] pktcol']]; easy.
+      -- destruct d_wf as [[col [colgy [pgy sgy]]] [[psy pkt_wf] [ccc c_wf]]].
+         destruct col; unfold green_or_yellow in colgy; easy.
+Qed.
